<?xml version="1.0"?>


<!DOCTYPE rdf:RDF [
    <!ENTITY owl "http://www.w3.org/2002/07/owl#" >
    <!ENTITY xsd "http://www.w3.org/2001/XMLSchema#" >
    <!ENTITY skos "http://www.w3.org/2004/02/skos/core#" >
    <!ENTITY rdfs "http://www.w3.org/2000/01/rdf-schema#" >
    <!ENTITY rdf "http://www.w3.org/1999/02/22-rdf-syntax-ns#" >
    <!ENTITY schemas "http://sustainablesourcing.ucdavis.edu/schemas/" >
    <!ENTITY asi "http://asi.ice.ucdavis.edu/sustsource/schemas/sustsource.owl#" >
    <!ENTITY sustsource "http://sustainablesourcing.ucdavis.edu/schemas/sustsource.owl#" >
]>


<rdf:RDF xmlns="http://asi.ice.ucdavis.edu/sustsource/schemas/sustsource.owl#"
     xml:base="http://asi.ice.ucdavis.edu/sustsource/schemas/sustsource.owl"
     xmlns:rdfs="http://www.w3.org/2000/01/rdf-schema#"
     xmlns:schemas="http://sustainablesourcing.ucdavis.edu/schemas/"
     xmlns:asi="http://asi.ice.ucdavis.edu/sustsource/schemas/sustsource.owl#"
     xmlns:owl="http://www.w3.org/2002/07/owl#"
     xmlns:xsd="http://www.w3.org/2001/XMLSchema#"
     xmlns:rdf="http://www.w3.org/1999/02/22-rdf-syntax-ns#"
     xmlns:skos="http://www.w3.org/2004/02/skos/core#"
     xmlns:sustsource="&schemas;sustsource.owl#">
    <owl:Ontology rdf:about="http://asi.ice.ucdavis.edu/sustsource/sustsource.owl#">
        <owl:versionInfo>Got Dublin Core properties from Simon Reinhardt OWL 2 DL version</owl:versionInfo>
        <owl:imports rdf:resource="http://purl.org/NET/dc_owl2dl/terms_od"/>
        <owl:imports rdf:resource="http://www.w3.org/2004/02/skos/core"/>
    </owl:Ontology>
    


    <!-- 
    ///////////////////////////////////////////////////////////////////////////////////////
    //
    // Annotation properties
    //
    ///////////////////////////////////////////////////////////////////////////////////////
     -->

    


    <!-- 
    ///////////////////////////////////////////////////////////////////////////////////////
    //
    // Datatypes
    //
    ///////////////////////////////////////////////////////////////////////////////////////
     -->

    


    <!-- 
    ///////////////////////////////////////////////////////////////////////////////////////
    //
    // Object Properties
    //
    ///////////////////////////////////////////////////////////////////////////////////////
     -->

    


    <!-- http://asi.ice.ucdavis.edu/sustsource/schemas/sustsource.owl#fullyCovers -->

    <owl:ObjectProperty rdf:about="&asi;fullyCovers">
        <rdfs:label>Fully covers</rdfs:label>
        <rdfs:comment>A link showing that an indicator fully covers (at least at the 80% level) a particular issue.</rdfs:comment>
        <rdfs:domain rdf:resource="&asi;Indicator"/>
        <rdfs:domain rdf:resource="&asi;IndicatorGroup"/>
        <rdfs:range rdf:resource="&asi;Issue"/>
    </owl:ObjectProperty>
    


    <!-- http://asi.ice.ucdavis.edu/sustsource/schemas/sustsource.owl#hasMeasurementScale -->

    <owl:ObjectProperty rdf:about="&asi;hasMeasurementScale">
        <rdfs:label>Has measurement scale</rdfs:label>
        <rdfs:domain rdf:resource="&asi;Indicator"/>
        <rdfs:range rdf:resource="&asi;Scale"/>
    </owl:ObjectProperty>
    


    <!-- http://asi.ice.ucdavis.edu/sustsource/schemas/sustsource.owl#hasReportingScale -->

    <owl:ObjectProperty rdf:about="&asi;hasReportingScale">
        <rdfs:label>Has reporting scale</rdfs:label>
    </owl:ObjectProperty>
    


    <!-- http://asi.ice.ucdavis.edu/sustsource/schemas/sustsource.owl#inFramework -->

    <owl:ObjectProperty rdf:about="&asi;inFramework">
        <rdfs:label>In framework</rdfs:label>
    </owl:ObjectProperty>
    


    <!-- http://asi.ice.ucdavis.edu/sustsource/schemas/sustsource.owl#partiallyCovers -->

    <owl:ObjectProperty rdf:about="&asi;partiallyCovers">
        <rdfs:label>Partially covers</rdfs:label>
        <rdfs:comment>The link shows that the indicator partially covers the issue.</rdfs:comment>
        <rdfs:domain rdf:resource="&asi;Indicator"/>
        <rdfs:domain rdf:resource="&asi;IndicatorGroup"/>
        <rdfs:range rdf:resource="&asi;Issue"/>
    </owl:ObjectProperty>
    


    <!-- 
    ///////////////////////////////////////////////////////////////////////////////////////
    //
    // Data properties
    //
    ///////////////////////////////////////////////////////////////////////////////////////
     -->

    


    <!-- http://asi.ice.ucdavis.edu/sustsource/schemas/sustsource.owl#citationKey -->

    <owl:DatatypeProperty rdf:about="&asi;citationKey">
        <rdfs:label>Citation key</rdfs:label>
    </owl:DatatypeProperty>
    


    <!-- http://asi.ice.ucdavis.edu/sustsource/schemas/sustsource.owl#firstname -->

    <owl:DatatypeProperty rdf:about="&asi;firstname">
        <rdfs:label>First name</rdfs:label>
        <rdfs:domain rdf:resource="&asi;Person"/>
        <rdfs:range rdf:resource="&xsd;string"/>
    </owl:DatatypeProperty>
    


    <!-- http://asi.ice.ucdavis.edu/sustsource/schemas/sustsource.owl#fullname -->

    <owl:DatatypeProperty rdf:about="&asi;fullname">
        <rdfs:label>Full name</rdfs:label>
        <rdfs:domain rdf:resource="&asi;Person"/>
        <rdfs:range rdf:resource="&xsd;string"/>
    </owl:DatatypeProperty>
    


    <!-- http://asi.ice.ucdavis.edu/sustsource/schemas/sustsource.owl#hasUnits -->

    <owl:DatatypeProperty rdf:about="&asi;hasUnits">
        <rdfs:label>Has units</rdfs:label>
    </owl:DatatypeProperty>
    


    <!-- http://asi.ice.ucdavis.edu/sustsource/schemas/sustsource.owl#issueVerbatim -->

    <owl:DatatypeProperty rdf:about="&asi;issueVerbatim">
        <rdfs:label>Issue - verbatim</rdfs:label>
        <rdfs:comment>Verbatim encoding of issue in reference source</rdfs:comment>
        <rdfs:domain rdf:resource="&asi;Indicator"/>
    </owl:DatatypeProperty>
    


    <!-- http://asi.ice.ucdavis.edu/sustsource/schemas/sustsource.owl#middlename -->

    <owl:DatatypeProperty rdf:about="&asi;middlename">
        <rdfs:label>Middle name</rdfs:label>
        <rdfs:domain rdf:resource="&asi;Person"/>
        <rdfs:range rdf:resource="&xsd;string"/>
    </owl:DatatypeProperty>
    


    <!-- http://asi.ice.ucdavis.edu/sustsource/schemas/sustsource.owl#orgabbrev -->

    <owl:DatatypeProperty rdf:about="&asi;orgabbrev">
        <rdfs:label>Organization abbreviation</rdfs:label>
        <rdfs:domain rdf:resource="&asi;Organization"/>
        <rdfs:range rdf:resource="&xsd;string"/>
        <rdfs:subPropertyOf rdf:resource="&owl;topDataProperty"/>
    </owl:DatatypeProperty>
    


    <!-- http://asi.ice.ucdavis.edu/sustsource/schemas/sustsource.owl#orglocation -->

    <owl:DatatypeProperty rdf:about="&asi;orglocation">
        <rdfs:label>Organization location</rdfs:label>
        <rdfs:domain rdf:resource="&asi;Organization"/>
        <rdfs:range rdf:resource="&xsd;string"/>
    </owl:DatatypeProperty>
    


    <!-- http://asi.ice.ucdavis.edu/sustsource/schemas/sustsource.owl#orgname -->

    <owl:DatatypeProperty rdf:about="&asi;orgname">
        <rdfs:label>Organization name</rdfs:label>
        <rdfs:domain rdf:resource="&asi;Organization"/>
        <rdfs:range rdf:resource="&xsd;string"/>
    </owl:DatatypeProperty>
    


    <!-- http://asi.ice.ucdavis.edu/sustsource/schemas/sustsource.owl#surname -->

    <owl:DatatypeProperty rdf:about="&asi;surname">
        <rdfs:label>Surname</rdfs:label>
        <rdfs:domain rdf:resource="&asi;Person"/>
        <rdfs:range rdf:resource="&xsd;string"/>
    </owl:DatatypeProperty>
    


    <!-- 
    ///////////////////////////////////////////////////////////////////////////////////////
    //
    // Classes
    //
    ///////////////////////////////////////////////////////////////////////////////////////
     -->

    


    <!-- http://asi.ice.ucdavis.edu/sustsource/schemas/sustsource.owl#Capital -->

    <owl:Class rdf:about="&asi;Capital">
        <rdfs:label>Six capitals</rdfs:label>
        <rdfs:comment>We distinguish between the six capitals, and our main list of issue. Capitals are not issues, have addressed this in this version.</rdfs:comment>
    </owl:Class>
    


    <!-- http://asi.ice.ucdavis.edu/sustsource/schemas/sustsource.owl#City -->

    <owl:Class rdf:about="&asi;City">
        <rdfs:label>City</rdfs:label>
        <rdfs:subClassOf rdf:resource="&asi;Scale"/>
    </owl:Class>
    


    <!-- http://asi.ice.ucdavis.edu/sustsource/schemas/sustsource.owl#Community -->

    <owl:Class rdf:about="&asi;Community">
        <rdfs:label>Community</rdfs:label>
        <rdfs:subClassOf rdf:resource="&asi;Scale"/>
    </owl:Class>
    


    <!-- http://asi.ice.ucdavis.edu/sustsource/schemas/sustsource.owl#ComponentIssue -->

    <owl:Class rdf:about="&asi;ComponentIssue">
        <rdfs:label>Component issue</rdfs:label>
        <rdfs:subClassOf rdf:resource="&asi;Issue"/>
        <rdfs:comment>Component issues were created to subdivide integrated issues to provide a better impendance match to the indicators. They are mostly taken from AGROVOC.</rdfs:comment>
    </owl:Class>
    


    <!-- http://asi.ice.ucdavis.edu/sustsource/schemas/sustsource.owl#CoreIssue -->

    <owl:Class rdf:about="&asi;CoreIssue">
        <rdfs:label>Core issue</rdfs:label>
        <rdfs:subClassOf rdf:resource="&asi;Issue"/>
    </owl:Class>
    


    <!-- http://asi.ice.ucdavis.edu/sustsource/schemas/sustsource.owl#Country -->

    <owl:Class rdf:about="&asi;Country">
        <rdfs:label>Country</rdfs:label>
        <rdfs:subClassOf rdf:resource="&asi;Scale"/>
    </owl:Class>
    


    <!-- http://asi.ice.ucdavis.edu/sustsource/schemas/sustsource.owl#County -->

    <owl:Class rdf:about="&asi;County">
        <rdfs:label>County</rdfs:label>
        <rdfs:subClassOf rdf:resource="&asi;Scale"/>
    </owl:Class>
    


    <!-- http://asi.ice.ucdavis.edu/sustsource/schemas/sustsource.owl#DataType -->

    <owl:Class rdf:about="&asi;DataType">
        <rdfs:label>Data type</rdfs:label>
    </owl:Class>
    


    <!-- http://asi.ice.ucdavis.edu/sustsource/schemas/sustsource.owl#Farm -->

    <owl:Class rdf:about="&asi;Farm">
        <rdfs:label>Farm</rdfs:label>
        <rdfs:subClassOf rdf:resource="&asi;Scale"/>
    </owl:Class>
    


    <!-- http://asi.ice.ucdavis.edu/sustsource/schemas/sustsource.owl#Framework -->

    <owl:Class rdf:about="&asi;Framework">
        <rdfs:label>Framework</rdfs:label>
    </owl:Class>
    


    <!-- http://asi.ice.ucdavis.edu/sustsource/schemas/sustsource.owl#Global -->

    <owl:Class rdf:about="&asi;Global">
        <rdfs:label>Global</rdfs:label>
        <rdfs:subClassOf rdf:resource="&asi;Scale"/>
    </owl:Class>
    


    <!-- http://asi.ice.ucdavis.edu/sustsource/schemas/sustsource.owl#Household -->

    <owl:Class rdf:about="&asi;Household">
        <rdfs:label>Household</rdfs:label>
        <rdfs:subClassOf rdf:resource="&asi;Scale"/>
    </owl:Class>
    


    <!-- http://asi.ice.ucdavis.edu/sustsource/schemas/sustsource.owl#Indicator -->

    <owl:Class rdf:about="&asi;Indicator">
        <rdfs:label>Indicator</rdfs:label>
        <rdfs:comment>indicatorverbatim -&gt; dc:title</rdfs:comment>
    </owl:Class>
    


    <!-- http://asi.ice.ucdavis.edu/sustsource/schemas/sustsource.owl#IndicatorGroup -->

    <owl:Class rdf:about="&asi;IndicatorGroup">
        <rdfs:label>Indicator group</rdfs:label>
        <rdfs:comment>A group of indicators related for some purpose. In general these will not have any identity more than a convenience identifier (&quot;IndGroup1&quot;), One use is to label a set of indicators that together fully cover an issue.</rdfs:comment>
    </owl:Class>
    


    <!-- http://asi.ice.ucdavis.edu/sustsource/schemas/sustsource.owl#Individual -->

    <owl:Class rdf:about="&asi;Individual">
        <rdfs:label>Individual</rdfs:label>
        <rdfs:subClassOf rdf:resource="&asi;Scale"/>
    </owl:Class>
    


    <!-- http://asi.ice.ucdavis.edu/sustsource/schemas/sustsource.owl#IntegratedIssue -->

    <owl:Class rdf:about="&asi;IntegratedIssue">
        <rdfs:label>Integrated issue</rdfs:label>
        <rdfs:subClassOf rdf:resource="&asi;Issue"/>
        <rdfs:comment>One of our core list of issues. Most of these come from AGROVOC,
put in links at some point.</rdfs:comment>
    </owl:Class>
    


    <!-- http://asi.ice.ucdavis.edu/sustsource/schemas/sustsource.owl#Issue -->

    <owl:Class rdf:about="&asi;Issue">
        <rdfs:label>Issue</rdfs:label>
    </owl:Class>
    


    <!-- http://asi.ice.ucdavis.edu/sustsource/schemas/sustsource.owl#MulticountryRegion -->

    <owl:Class rdf:about="&asi;MulticountryRegion">
        <rdfs:label>Multicountry region</rdfs:label>
        <rdfs:subClassOf rdf:resource="&asi;Scale"/>
    </owl:Class>
    


    <!-- http://asi.ice.ucdavis.edu/sustsource/schemas/sustsource.owl#Organization -->

    <owl:Class rdf:about="&asi;Organization">
        <rdfs:label>Organization</rdfs:label>
    </owl:Class>
    


    <!-- http://asi.ice.ucdavis.edu/sustsource/schemas/sustsource.owl#Person -->

    <owl:Class rdf:about="&asi;Person">
        <rdfs:label>Person</rdfs:label>
        <rdfs:comment>Clearly can find a better URI for this. Could just use FOAF.</rdfs:comment>
    </owl:Class>
    


    <!-- http://asi.ice.ucdavis.edu/sustsource/schemas/sustsource.owl#PhysicalFinancialCapital -->

    <owl:Class rdf:about="&asi;PhysicalFinancialCapital">
        <rdfs:label>Physical &amp; Financial Capital</rdfs:label>
        <rdfs:subClassOf rdf:resource="&asi;Capital"/>
    </owl:Class>
    


    <!-- http://asi.ice.ucdavis.edu/sustsource/schemas/sustsource.owl#Region -->

    <owl:Class rdf:about="&asi;Region">
        <rdfs:label>Region</rdfs:label>
        <rdfs:subClassOf rdf:resource="&asi;Scale"/>
    </owl:Class>
    


    <!-- http://asi.ice.ucdavis.edu/sustsource/schemas/sustsource.owl#Scale -->

    <owl:Class rdf:about="&asi;Scale">
        <rdfs:label>Scale</rdfs:label>
    </owl:Class>
    


    <!-- http://asi.ice.ucdavis.edu/sustsource/schemas/sustsource.owl#SocialPoliticalCapital -->

    <owl:Class rdf:about="&asi;SocialPoliticalCapital">
        <rdfs:label>Social &amp; Political Capital</rdfs:label>
        <rdfs:subClassOf rdf:resource="&asi;Capital"/>
    </owl:Class>
    


    <!-- http://asi.ice.ucdavis.edu/sustsource/schemas/sustsource.owl#Strategy -->

    <owl:Class rdf:about="&asi;Strategy">
        <rdfs:label>Strategy</rdfs:label>
    </owl:Class>
    


    <!-- http://asi.ice.ucdavis.edu/sustsource/schemas/sustsource.owl#Village -->

    <owl:Class rdf:about="&asi;Village">
        <rdfs:label>Village</rdfs:label>
        <rdfs:subClassOf rdf:resource="&asi;Scale"/>
    </owl:Class>
    


    <!-- http://asi.ice.ucdavis.edu/sustsource/schemas/sustsource.owl#Watershed -->

    <owl:Class rdf:about="&asi;Watershed">
        <rdfs:label>Watershed</rdfs:label>
        <rdfs:subClassOf rdf:resource="&asi;Scale"/>
    </owl:Class>
    


    <!-- http://purl.org/dc/terms/BibliographicResource -->

    <rdf:Description rdf:about="http://purl.org/dc/terms/BibliographicResource">
        <rdfs:comment>Most terms in original source database model represented in dcterms, viz:
title: dc:title
creator: dc:creator
dateofsource: dc:created-003 etc.
*citationkey: probably need to add
URL: dc:identifier
subjectclassification: use SKOS reference
subjectterm: use SKOS reference
*resourcetype: probably should add
spatialcoverage: DC
temporalcoverage: DC
personalauthor:
corporateauthor: dc:creator, don&apos;t worry about distinction
contributor: DC
publisher: DC
organization: find good usage. FOAF?
journal: this is to go into AGRIS, right? not sure
citation: dcterms:bibliographicCiation
dateaccessed: not in dc?
relation: dc,
format: dc
language: dc
rights: dc
suitability: add term
funding: add term
design: add term
inclusion: add term
notes: add term
mendeleyURL: leave out for now
AGRISready: leave out for now

</rdfs:comment>
        <owl:hasKey rdf:parseType="Collection">
            <rdf:Description rdf:about="&asi;citationKey"/>
        </owl:hasKey>
    </rdf:Description>
    


    <!-- 
    ///////////////////////////////////////////////////////////////////////////////////////
    //
    // Individuals
    //
    ///////////////////////////////////////////////////////////////////////////////////////
     -->

    


    <!-- http://asi.ice.ucdavis.edu/sustsource/schemas/sustsource.owl#AgriculturalSector -->

    <owl:NamedIndividual rdf:about="&asi;AgriculturalSector">
        <rdf:type rdf:resource="&asi;IntegratedIssue"/>
        <rdf:type rdf:resource="&skos;Concept"/>
        <rdfs:label>Agricultural sector</rdfs:label>
        <rdfs:comment>Refers to the role of agriculture in regional and national economies.</rdfs:comment>
        <skos:related rdf:resource="&asi;Disasters"/>
        <inFramework rdf:resource="&asi;ImpactMitigationFramework"/>
        <skos:related rdf:resource="&asi;Income"/>
        <skos:related rdf:resource="&asi;Inputs"/>
        <skos:related rdf:resource="&asi;Markets"/>
        <skos:related rdf:resource="&asi;PhysicalFinancialCapital"/>
        <skos:related rdf:resource="&asi;Productivity"/>
        <skos:related rdf:resource="&asi;TradePolicies"/>
        <inFramework rdf:resource="&asi;VulnerabilityResilienceFramework"/>
    </owl:NamedIndividual>
    


    <!-- http://asi.ice.ucdavis.edu/sustsource/schemas/sustsource.owl#AirAndClimate -->

    <owl:NamedIndividual rdf:about="&asi;AirAndClimate">
        <rdf:type rdf:resource="&asi;IntegratedIssue"/>
        <rdf:type rdf:resource="&skos;Concept"/>
        <rdfs:label>Air &amp; climate</rdfs:label>
        <rdfs:comment>GHG emissions, ozone layer depletion, air quality, climate change influenced and extreme weather events, shifts in growing zones for key crops due to climate change.</rdfs:comment>
        <skos:related rdf:resource="&asi;CommonPoolResources"/>
        <skos:related rdf:resource="&asi;Energy"/>
        <inFramework rdf:resource="&asi;ImpactMitigationFramework"/>
        <skos:related rdf:resource="&asi;Infrastructure"/>
        <skos:related rdf:resource="&asi;NaturalCapital"/>
        <inFramework rdf:resource="&asi;VulnerabilityResilienceFramework"/>
        <skos:related rdf:resource="&asi;WastesAndPollution"/>
    </owl:NamedIndividual>
    


    <!-- http://asi.ice.ucdavis.edu/sustsource/schemas/sustsource.owl#Biodiversity -->

    <owl:NamedIndividual rdf:about="&asi;Biodiversity">
        <rdf:type rdf:resource="&asi;IntegratedIssue"/>
        <rdf:type rdf:resource="&skos;Concept"/>
        <rdfs:label>Biodiversity</rdfs:label>
        <rdfs:comment>Number of total species, number of endemic species, species loss or introduction, species threatened with extinction or endangerment, trade in wildlife and captive-bred animal species, trophic integrity of ecosystems, extent of specific habitats (or extent of habitat fragmentation), biodiversity as a source of genetic pool for food/medicine. </rdfs:comment>
        <skos:related rdf:resource="&asi;CommonPoolResources"/>
        <skos:related rdf:resource="&asi;Deforestation"/>
        <skos:related rdf:resource="&asi;EcosystemServices"/>
        <inFramework rdf:resource="&asi;ImpactMitigationFramework"/>
        <skos:related rdf:resource="&asi;LandAndSoil"/>
        <skos:related rdf:resource="&asi;NaturalCapital"/>
        <skos:related rdf:resource="&asi;ProtectedAreas"/>
        <skos:related rdf:resource="&asi;TradePolicies"/>
    </owl:NamedIndividual>
    


    <!-- http://asi.ice.ucdavis.edu/sustsource/schemas/sustsource.owl#CommonPoolResources -->

    <owl:NamedIndividual rdf:about="&asi;CommonPoolResources">
        <rdf:type rdf:resource="&asi;IntegratedIssue"/>
        <rdf:type rdf:resource="&skos;Concept"/>
        <rdfs:label>Common pool resources</rdfs:label>
        <rdfs:comment>Resources that are not the private property of any individual or group, but rather are used by many people for their benefit.</rdfs:comment>
        <skos:related rdf:resource="&asi;AirAndClimate"/>
        <skos:related rdf:resource="&asi;Biodiversity"/>
        <skos:related rdf:resource="&asi;Deforestation"/>
        <skos:related rdf:resource="&asi;EcosystemServices"/>
        <skos:related rdf:resource="&asi;Governance"/>
        <inFramework rdf:resource="&asi;ImpactMitigationFramework"/>
        <skos:related rdf:resource="&asi;Institutions"/>
        <skos:related rdf:resource="&asi;LandAndSoil"/>
        <skos:related rdf:resource="&asi;NaturalCapital"/>
        <skos:related rdf:resource="&asi;OceansAndCoasts"/>
        <skos:related rdf:resource="&asi;PropertyRights"/>
        <skos:related rdf:resource="&asi;Water"/>
    </owl:NamedIndividual>
    


    <!-- http://asi.ice.ucdavis.edu/sustsource/schemas/sustsource.owl#Deforestation -->

    <owl:NamedIndividual rdf:about="&asi;Deforestation">
        <rdf:type rdf:resource="&asi;IntegratedIssue"/>
        <rdf:type rdf:resource="&skos;Concept"/>
        <rdfs:label>Deforestation</rdfs:label>
        <rdfs:comment>Removal of forest cover, and conversion to other uses including farming or grazing. Laws and regulations related to preventing deforestation and their enforcement.</rdfs:comment>
        <skos:related rdf:resource="&asi;Biodiversity"/>
        <skos:related rdf:resource="&asi;CommonPoolResources"/>
        <skos:related rdf:resource="&asi;EcosystemServices"/>
        <skos:related rdf:resource="&asi;Governance"/>
        <inFramework rdf:resource="&asi;ImpactMitigationFramework"/>
        <skos:related rdf:resource="&asi;LandAndSoil"/>
        <skos:related rdf:resource="&asi;NaturalCapital"/>
        <skos:related rdf:resource="&asi;PropertyRights"/>
        <inFramework rdf:resource="&asi;VulnerabilityResilienceFramework"/>
    </owl:NamedIndividual>
    


    <!-- http://asi.ice.ucdavis.edu/sustsource/schemas/sustsource.owl#Disasters -->

    <owl:NamedIndividual rdf:about="&asi;Disasters">
        <rdf:type rdf:resource="&asi;IntegratedIssue"/>
        <rdf:type rdf:resource="&skos;Concept"/>
        <rdfs:label>Disasters</rdfs:label>
        <rdfs:comment>Occurrence, frequency, and severity of natural disasters and human influenced disasters such as civil conflict and war, economic crises, and epidemics, in a given area. The number of people affected or projected to be affected, the risk of particular crop or growing region to disasters, and mechanisms for disaster resilience including governmental support and insurance are themes of this issue.</rdfs:comment>
        <skos:related rdf:resource="&asi;AgriculturalSector"/>
        <skos:related rdf:resource="&asi;AirAndClimate"/>
        <skos:related rdf:resource="&asi;Governance"/>
        <skos:related rdf:resource="&asi;Infrastructure"/>
        <skos:related rdf:resource="&asi;Institutions"/>
        <skos:related rdf:resource="&asi;Productivity"/>
        <skos:related rdf:resource="&asi;Safety"/>
        <skos:related rdf:resource="&asi;SocialPoliticalCapital"/>
        <inFramework rdf:resource="&asi;VulnerabilityResilienceFramework"/>
    </owl:NamedIndividual>
    


    <!-- http://asi.ice.ucdavis.edu/sustsource/schemas/sustsource.owl#Diseases -->

    <owl:NamedIndividual rdf:about="&asi;Diseases">
        <rdf:type rdf:resource="&asi;IntegratedIssue"/>
        <rdf:type rdf:resource="&skos;Concept"/>
        <rdfs:label>Diseases</rdfs:label>
        <rdfs:comment>Rates of incidence and information about transmission risks of diseases in a given area, or among a certain population. This issue relates to human diseases; diseases that affect plants or other animals are captured in food production and productivity or other issues.</rdfs:comment>
        <skos:related rdf:resource="&asi;HumanCapital"/>
        <skos:related rdf:resource="&asi;Mortality"/>
        <skos:related rdf:resource="&asi;PublicHealth"/>
        <skos:related rdf:resource="&asi;ReproductiveHealth"/>
        <skos:related rdf:resource="&asi;Safety"/>
        <inFramework rdf:resource="&asi;VulnerabilityResilienceFramework"/>
        <skos:related rdf:resource="&asi;Water"/>
    </owl:NamedIndividual>
    


    <!-- http://asi.ice.ucdavis.edu/sustsource/schemas/sustsource.owl#EcosystemServices -->

    <owl:NamedIndividual rdf:about="&asi;EcosystemServices">
        <rdf:type rdf:resource="&asi;IntegratedIssue"/>
        <rdf:type rdf:resource="&skos;Concept"/>
        <rdfs:label>Ecosystem services</rdfs:label>
        <rdfs:comment>The benefits people obtain from ecosystems. These include provisioning services such as food and water; regulating services such as flood and disease control; cultural services such as spiritual, recreational, and cultural benefits; and supporting services such as nutrient cycling that maintain the conditions for life on earth.</rdfs:comment>
        <skos:related rdf:resource="&asi;AirAndClimate"/>
        <skos:related rdf:resource="&asi;Biodiversity"/>
        <skos:related rdf:resource="&asi;CommonPoolResources"/>
        <inFramework rdf:resource="&asi;ImpactMitigationFramework"/>
        <skos:related rdf:resource="&asi;LandAndSoil"/>
        <skos:related rdf:resource="&asi;NaturalCapital"/>
        <skos:related rdf:resource="&asi;OceansAndCoasts"/>
        <skos:related rdf:resource="&asi;Productivity"/>
        <skos:related rdf:resource="&asi;ProtectedAreas"/>
        <inFramework rdf:resource="&asi;VulnerabilityResilienceFramework"/>
        <skos:related rdf:resource="&asi;Water"/>
    </owl:NamedIndividual>
    


    <!-- http://asi.ice.ucdavis.edu/sustsource/schemas/sustsource.owl#EducationalResources -->

    <owl:NamedIndividual rdf:about="&asi;EducationalResources">
        <rdf:type rdf:resource="&asi;IntegratedIssue"/>
        <rdf:type rdf:resource="&skos;Concept"/>
        <rdfs:label>Educational resources</rdfs:label>
        <rdfs:comment>Educational opportunities and achievement, with attention to gender-based access dimensions. Includes formal education, informal or traditional knowledge transfer, extension services, and vocational training, especially related to improved agricultural practices. Also includes access to legal, public, and reproductive health education services.</rdfs:comment>
        <skos:related rdf:resource="&asi;Literacy"/>
        <skos:related rdf:resource="&asi;NutritionalStatus"/>
        <skos:related rdf:resource="&asi;PublicHealth"/>
        <skos:related rdf:resource="&asi;ReproductiveHealth"/>
        <skos:related rdf:resource="&asi;SocialPoliticalCapital"/>
        <inFramework rdf:resource="&asi;VulnerabilityResilienceFramework"/>
    </owl:NamedIndividual>
    


    <!-- http://asi.ice.ucdavis.edu/sustsource/schemas/sustsource.owl#Energy -->

    <owl:NamedIndividual rdf:about="&asi;Energy">
        <rdf:type rdf:resource="&asi;IntegratedIssue"/>
        <rdf:type rdf:resource="&skos;Concept"/>
        <rdfs:label>Energy</rdfs:label>
        <rdfs:comment>Proportion and type of renewable or fossil fuel used for energy production, emissions and other impacts associated with energy production, prices of energy by type and as a proportion of household income; access to energy - including liquid fuel, gas, and electricity; energy production and distribution infrastructures; energy regulations, policies, and their enforcement.</rdfs:comment>
        <skos:related rdf:resource="&asi;AirAndClimate"/>
        <skos:related rdf:resource="&asi;Governance"/>
        <skos:related rdf:resource="&asi;Income"/>
        <skos:related rdf:resource="&asi;Infrastructure"/>
        <skos:related rdf:resource="&asi;PhysicalFinancialCapital"/>
        <skos:related rdf:resource="&asi;Poverty"/>
        <inFramework rdf:resource="&asi;VulnerabilityResilienceFramework"/>
    </owl:NamedIndividual>
    


    <!-- http://asi.ice.ucdavis.edu/sustsource/schemas/sustsource.owl#Finance -->

    <owl:NamedIndividual rdf:about="&asi;Finance">
        <rdf:type rdf:resource="&asi;IntegratedIssue"/>
        <rdf:type rdf:resource="&skos;Concept"/>
        <rdfs:label>Finance</rdfs:label>
        <rdfs:comment>Access to financial capital including loans, equity investments, and grants; reliable secured savings systems; crop or production insurance against risk, associated costs, and interest rates.</rdfs:comment>
        <skos:related rdf:resource="&asi;Governance"/>
        <skos:related rdf:resource="&asi;Income"/>
        <skos:related rdf:resource="&asi;Institutions"/>
        <skos:related rdf:resource="&asi;PhysicalFinancialCapital"/>
        <skos:related rdf:resource="&asi;TradePolicies"/>
        <inFramework rdf:resource="&asi;VulnerabilityResilienceFramework"/>
    </owl:NamedIndividual>
    


    <!-- http://asi.ice.ucdavis.edu/sustsource/schemas/sustsource.owl#FinancialCapital -->

    <owl:NamedIndividual rdf:about="&asi;FinancialCapital">
        <rdf:type rdf:resource="&asi;PhysicalFinancialCapital"/>
        <rdfs:label>Financial capital</rdfs:label>
        <rdfs:comment>The financial resources that people use to achieve their livelihood objectives.</rdfs:comment>
    </owl:NamedIndividual>
    


    <!-- http://asi.ice.ucdavis.edu/sustsource/schemas/sustsource.owl#FoodProduction -->

    <owl:NamedIndividual rdf:about="&asi;FoodProduction">
        <rdf:type rdf:resource="&asi;IntegratedIssue"/>
        <rdf:type rdf:resource="&skos;Concept"/>
        <rdfs:label>Food production</rdfs:label>
        <rdfs:comment>Food produced for direct human consumption; the ratio of cash crops to staple crops or biofuels to food crops Includes food availability and access to a nutritious and culturally acceptable range of food products. Also relates to stability or stochasticity in food access, food prices, and the policies, initiatives, and regulations to support agroecological systems.</rdfs:comment>
        <skos:related rdf:resource="&asi;EducationalResources"/>
        <skos:related rdf:resource="&asi;Governance"/>
        <skos:related rdf:resource="&asi;HumanRights"/>
        <inFramework rdf:resource="&asi;ImpactMitigationFramework"/>
        <skos:related rdf:resource="&asi;LandAndSoil"/>
        <skos:related rdf:resource="&asi;Markets"/>
        <skos:related rdf:resource="&asi;NutritionalStatus"/>
        <skos:related rdf:resource="&asi;Poverty"/>
        <skos:related rdf:resource="&asi;Productivity"/>
        <skos:related rdf:resource="&asi;PropertyRights"/>
        <skos:related rdf:resource="&asi;PublicHealth"/>
        <skos:related rdf:resource="&asi;SocialPoliticalCapital"/>
        <skos:related rdf:resource="&asi;TradePolicies"/>
        <inFramework rdf:resource="&asi;VulnerabilityResilienceFramework"/>
        <skos:related rdf:resource="&asi;Water"/>
    </owl:NamedIndividual>
    


    <!-- http://asi.ice.ucdavis.edu/sustsource/schemas/sustsource.owl#GeographicalDistribution -->

    <owl:NamedIndividual rdf:about="&asi;GeographicalDistribution">
        <rdf:type rdf:resource="&asi;IntegratedIssue"/>
        <rdf:type rdf:resource="&skos;Concept"/>
        <rdfs:label>Geographical distribution</rdfs:label>
        <rdfs:comment>Describes the proportions of total population (often at a national or broader level) that live in rural, suburban, and urban areas; densities of populations across different agro-ecological zones; and seasonal or other forms of migration (may include different/additional geographical classifications).</rdfs:comment>
        <skos:related rdf:resource="&asi;Income"/>
        <skos:related rdf:resource="&asi;Infrastructure"/>
        <skos:related rdf:resource="&asi;Labor"/>
        <skos:related rdf:resource="&asi;PopulationGrowth"/>
        <skos:related rdf:resource="&asi;PopulationStructure"/>
        <skos:related rdf:resource="&asi;Poverty"/>
        <skos:related rdf:resource="&asi;SocialPoliticalCapital"/>
        <skos:related rdf:resource="&asi;SocialStructure"/>
        <inFramework rdf:resource="&asi;VulnerabilityResilienceFramework"/>
    </owl:NamedIndividual>
    


    <!-- http://asi.ice.ucdavis.edu/sustsource/schemas/sustsource.owl#Governance -->

    <owl:NamedIndividual rdf:about="&asi;Governance">
        <rdf:type rdf:resource="&asi;IntegratedIssue"/>
        <rdf:type rdf:resource="&skos;Concept"/>
        <rdfs:label>Governance</rdfs:label>
        <rdfs:comment>Organizational management, decision-making structure for rules, laws, regulations, and policies across scales and levels. Emphases include diversity and representation of stakeholders involved in decision making and governance; transparency and accessibility of mechanisms for dispute resolution; and enforcement policies and procedures.</rdfs:comment>
        <inFramework rdf:resource="&asi;ImpactMitigationFramework"/>
        <skos:related rdf:resource="&asi;Labor"/>
        <skos:related rdf:resource="&asi;Participation"/>
        <skos:related rdf:resource="&asi;SocialPoliticalCapital"/>
        <skos:related rdf:resource="&asi;SocialStructure"/>
        <skos:related rdf:resource="&asi;SocioculturalSystems"/>
        <skos:related rdf:resource="&asi;TradePolicies"/>
        <inFramework rdf:resource="&asi;VulnerabilityResilienceFramework"/>
        <skos:related rdf:resource="&asi;WomensParticipation"/>
    </owl:NamedIndividual>
    


    <!-- http://asi.ice.ucdavis.edu/sustsource/schemas/sustsource.owl#HumanCapital -->

    <owl:NamedIndividual rdf:about="&asi;HumanCapital">
        <rdf:type rdf:resource="&asi;Capital"/>
        <rdf:type rdf:resource="&skos;Concept"/>
        <rdfs:label>Human capital</rdfs:label>
        <rdfs:comment>Human capital: skills, knowledge, ability to labor, and good health that enable people to achieve their livelihood objectives. Human capital is often linked to labor and is shaped by household size, skill level, leadership potential, health status, and other factors</rdfs:comment>
    </owl:NamedIndividual>
    


    <!-- http://asi.ice.ucdavis.edu/sustsource/schemas/sustsource.owl#HumanRights -->

    <owl:NamedIndividual rdf:about="&asi;HumanRights">
        <rdf:type rdf:resource="&asi;IntegratedIssue"/>
        <rdf:type rdf:resource="&skos;Concept"/>
        <rdfs:label>Human rights</rdfs:label>
        <rdfs:comment>Respect for human rights to life, liberty, non-discrimination, privacy, freedom of movement, marriage, property ownership, thought, religion, fair remuneration, safe and dignified working conditions, association, education, food, and all other rights applicable at national, regional, local, and global levels.</rdfs:comment>
        <inFramework rdf:resource="&asi;ImpactMitigationFramework"/>
        <skos:related rdf:resource="&asi;Institutions"/>
        <skos:related rdf:resource="&asi;Labor"/>
        <skos:related rdf:resource="&asi;Participation"/>
        <skos:related rdf:resource="&asi;SocialPoliticalCapital"/>
        <skos:related rdf:resource="&asi;SocialStructure"/>
        <inFramework rdf:resource="&asi;VulnerabilityResilienceFramework"/>
        <skos:related rdf:resource="&asi;WomensParticipation"/>
    </owl:NamedIndividual>
    


    <!-- http://asi.ice.ucdavis.edu/sustsource/schemas/sustsource.owl#ImpactMitigationFramework -->

    <owl:NamedIndividual rdf:about="&asi;ImpactMitigationFramework">
        <rdf:type rdf:resource="&asi;Framework"/>
        <rdfs:label>Impact/mitigation framework</rdfs:label>
    </owl:NamedIndividual>
    


    <!-- http://asi.ice.ucdavis.edu/sustsource/schemas/sustsource.owl#Income -->

    <owl:NamedIndividual rdf:about="&asi;Income">
        <rdf:type rdf:resource="&asi;IntegratedIssue"/>
        <rdf:type rdf:resource="&skos;Concept"/>
        <rdfs:label>Income</rdfs:label>
        <rdfs:comment>Adequacy, stability, and dependability of financial flows from labor, investment, rents, and goods sold - particularly among primary producers of agricultural raw materials.</rdfs:comment>
        <skos:related rdf:resource="&asi;AgriculturalSector"/>
        <skos:related rdf:resource="&asi;Finance"/>
        <inFramework rdf:resource="&asi;ImpactMitigationFramework"/>
        <skos:related rdf:resource="&asi;Inputs"/>
        <skos:related rdf:resource="&asi;Labor"/>
        <skos:related rdf:resource="&asi;PhysicalFinancialCapital"/>
        <skos:related rdf:resource="&asi;Poverty"/>
        <skos:related rdf:resource="&asi;Productivity"/>
        <skos:related rdf:resource="&asi;Technology"/>
        <inFramework rdf:resource="&asi;VulnerabilityResilienceFramework"/>
        <skos:related rdf:resource="&asi;WomenAndWages"/>
    </owl:NamedIndividual>
    


    <!-- http://asi.ice.ucdavis.edu/sustsource/schemas/sustsource.owl#Infrastructure -->

    <owl:NamedIndividual rdf:about="&asi;Infrastructure">
        <rdf:type rdf:resource="&asi;IntegratedIssue"/>
        <rdf:type rdf:resource="&skos;Concept"/>
        <rdfs:label>Infrastructure</rdfs:label>
        <rdfs:comment>Existence, maintenance, quality, and accessibility of physical and manufactured capital needed to support livelihoods, economies, natural resource management, and ecosystem sustainability. Includes transportation systems; water supply, storage, and sanitation facilities; energy-related infrastructure; and communications infrastructure. </rdfs:comment>
        <skos:related rdf:resource="&asi;Energy"/>
        <skos:related rdf:resource="&asi;Governance"/>
        <skos:related rdf:resource="&asi;Institutions"/>
        <skos:related rdf:resource="&asi;PhysicalFinancialCapital"/>
        <skos:related rdf:resource="&asi;PublicHealth"/>
        <skos:related rdf:resource="&asi;Technology"/>
        <inFramework rdf:resource="&asi;VulnerabilityResilienceFramework"/>
        <skos:related rdf:resource="&asi;Water"/>
    </owl:NamedIndividual>
    


    <!-- http://asi.ice.ucdavis.edu/sustsource/schemas/sustsource.owl#Inputs -->

    <owl:NamedIndividual rdf:about="&asi;Inputs">
        <rdf:type rdf:resource="&asi;IntegratedIssue"/>
        <rdf:type rdf:resource="&skos;Concept"/>
        <rdfs:label>Inputs</rdfs:label>
        <rdfs:comment>Availability, accessibility, adequacy, and/or responsible use of chemical and organic fertilizer, insecticides, fungicides, and improved seed varieties.</rdfs:comment>
        <skos:related rdf:resource="&asi;AgriculturalSector"/>
        <skos:related rdf:resource="&asi;Finance"/>
        <skos:related rdf:resource="&asi;FoodProduction"/>
        <skos:related rdf:resource="&asi;Income"/>
        <skos:related rdf:resource="&asi;Labor"/>
        <skos:related rdf:resource="&asi;PhysicalFinancialCapital"/>
        <skos:related rdf:resource="&asi;Poverty"/>
        <skos:related rdf:resource="&asi;Productivity"/>
        <skos:related rdf:resource="&asi;Technology"/>
        <inFramework rdf:resource="&asi;VulnerabilityResilienceFramework"/>
        <skos:related rdf:resource="&asi;WastesAndPollution"/>
        <skos:related rdf:resource="&asi;Water"/>
    </owl:NamedIndividual>
    


    <!-- http://asi.ice.ucdavis.edu/sustsource/schemas/sustsource.owl#Institutions -->

    <owl:NamedIndividual rdf:about="&asi;Institutions">
        <rdf:type rdf:resource="&asi;IntegratedIssue"/>
        <rdf:type rdf:resource="&skos;Concept"/>
        <rdfs:label>Institutions</rdfs:label>
        <rdfs:comment>&quot;Institutions are the humanly devised constraints that structure political, economic and social interaction. They consist of both informal constraints (sanctions, taboos, customs, traditions, and codes of conduct), and formal rules (constitutions, laws, property rights). Throughout history, institutions have been devised by human beings to create order and reduce uncertainty in exchange&quot; (D.C. North, 1991. J. Economic Perspectives 5:97-112). We focus on the institutions at many levels that affect the food and agriculture supply chain.</rdfs:comment>
        <skos:related rdf:resource="&asi;Governance"/>
        <skos:related rdf:resource="&asi;HumanRights"/>
        <skos:related rdf:resource="&asi;Labor"/>
        <skos:related rdf:resource="&asi;Markets"/>
        <skos:related rdf:resource="&asi;Participation"/>
        <skos:related rdf:resource="&asi;SocialPoliticalCapital"/>
        <skos:related rdf:resource="&asi;TradePolicies"/>
        <inFramework rdf:resource="&asi;VulnerabilityResilienceFramework"/>
    </owl:NamedIndividual>
    


    <!-- http://asi.ice.ucdavis.edu/sustsource/schemas/sustsource.owl#Labor -->

    <owl:NamedIndividual rdf:about="&asi;Labor">
        <rdf:type rdf:resource="&asi;IntegratedIssue"/>
        <rdf:type rdf:resource="&skos;Concept"/>
        <rdfs:label>Labor</rdfs:label>
        <rdfs:comment>Includes employment and labor conditions in the agricultural production sector, as well as dynamics that affect labor relations such as landholding size, crop production type, and wealth status. Also includes issues of access to labor, i.e. are there enough employable people in a given production system to maximize productivity.</rdfs:comment>
        <skos:related rdf:resource="&asi;GeographicalDistribution"/>
        <skos:related rdf:resource="&asi;Governance"/>
        <skos:related rdf:resource="&asi;HumanCapital"/>
        <skos:related rdf:resource="&asi;HumanRights"/>
        <inFramework rdf:resource="&asi;ImpactMitigationFramework"/>
        <skos:related rdf:resource="&asi;Institutions"/>
        <skos:related rdf:resource="&asi;Participation"/>
        <skos:related rdf:resource="&asi;Productivity"/>
        <inFramework rdf:resource="&asi;VulnerabilityResilienceFramework"/>
        <skos:related rdf:resource="&asi;WomenAndWages"/>
    </owl:NamedIndividual>
    


    <!-- http://asi.ice.ucdavis.edu/sustsource/schemas/sustsource.owl#LandAndSoil -->

    <owl:NamedIndividual rdf:about="&asi;LandAndSoil">
        <rdf:type rdf:resource="&asi;IntegratedIssue"/>
        <rdf:type rdf:resource="&skos;Concept"/>
        <rdfs:label>Land and soil</rdfs:label>
        <rdfs:comment>Characteristics of and changes in land use, land cover, soil quality. Connected themes include crop yield, production practices, characteristics of arable or pasture land, erosion, desertification, and measures of habitat fragmentation and connectivity.</rdfs:comment>
        <skos:related rdf:resource="&asi;Biodiversity"/>
        <skos:related rdf:resource="&asi;Deforestation"/>
        <skos:related rdf:resource="&asi;EcosystemServices"/>
        <skos:related rdf:resource="&asi;FoodProduction"/>
        <inFramework rdf:resource="&asi;ImpactMitigationFramework"/>
        <skos:related rdf:resource="&asi;NaturalCapital"/>
        <skos:related rdf:resource="&asi;Productivity"/>
        <skos:related rdf:resource="&asi;ProtectedAreas"/>
        <inFramework rdf:resource="&asi;VulnerabilityResilienceFramework"/>
    </owl:NamedIndividual>
    


    <!-- http://asi.ice.ucdavis.edu/sustsource/schemas/sustsource.owl#Literacy -->

    <owl:NamedIndividual rdf:about="&asi;Literacy">
        <rdf:type rdf:resource="&asi;IntegratedIssue"/>
        <rdf:type rdf:resource="&skos;Concept"/>
        <rdfs:label>Literacy</rdfs:label>
        <rdfs:comment>Rate of literacy in a given population, often classified by age group and gender.</rdfs:comment>
        <skos:related rdf:resource="&asi;EducationalResources"/>
        <skos:related rdf:resource="&asi;HumanCapital"/>
        <skos:related rdf:resource="&asi;SocioculturalSystems"/>
        <inFramework rdf:resource="&asi;VulnerabilityResilienceFramework"/>
    </owl:NamedIndividual>
    


    <!-- http://asi.ice.ucdavis.edu/sustsource/schemas/sustsource.owl#Markets -->

    <owl:NamedIndividual rdf:about="&asi;Markets">
        <rdf:type rdf:resource="&asi;IntegratedIssue"/>
        <rdf:type rdf:resource="&skos;Concept"/>
        <rdfs:label>Markets</rdfs:label>
        <rdfs:comment>Access to markets at local, regional, and global levels. Includes issues of fair pricing, price stability, knowledge transfer, and information to support negotiation and timing of transactions the number, role and communications among mid-supply chain actors. Includes policies to promote more equitable sourcing from small scale, historically underrepresented producers in global supply chains.</rdfs:comment>
        <skos:related rdf:resource="&asi;AgriculturalSector"/>
        <skos:related rdf:resource="&asi;Governance"/>
        <inFramework rdf:resource="&asi;ImpactMitigationFramework"/>
        <skos:related rdf:resource="&asi;Income"/>
        <skos:related rdf:resource="&asi;Institutions"/>
        <skos:related rdf:resource="&asi;Participation"/>
        <skos:related rdf:resource="&asi;SocialPoliticalCapital"/>
        <inFramework rdf:resource="&asi;VulnerabilityResilienceFramework"/>
        <skos:related rdf:resource="&asi;WomensParticipation"/>
    </owl:NamedIndividual>
    


    <!-- http://asi.ice.ucdavis.edu/sustsource/schemas/sustsource.owl#Mortality -->

    <owl:NamedIndividual rdf:about="&asi;Mortality">
        <rdf:type rdf:resource="&asi;IntegratedIssue"/>
        <rdf:type rdf:resource="&skos;Concept"/>
        <rdfs:label>Mortality</rdfs:label>
        <rdfs:comment>Average lifespan, rates of infant mortality, child mortality, maternal mortality in a given population.</rdfs:comment>
        <skos:related rdf:resource="&asi;Diseases"/>
        <skos:related rdf:resource="&asi;HumanCapital"/>
        <skos:related rdf:resource="&asi;PublicHealth"/>
        <skos:related rdf:resource="&asi;ReproductiveHealth"/>
    </owl:NamedIndividual>
    


    <!-- http://asi.ice.ucdavis.edu/sustsource/schemas/sustsource.owl#NaturalCapital -->

    <owl:NamedIndividual rdf:about="&asi;NaturalCapital">
        <rdf:type rdf:resource="&asi;Capital"/>
        <rdf:type rdf:resource="&skos;Concept"/>
        <rdfs:label>Natural capital</rdfs:label>
        <rdfs:comment>Natural resource stocks (e.g. nutrient cycling, erosion protection). Includes intangible public goods such as the atmosphere and biodiversity as well as divisible assets used for production (i.e. trees and land).</rdfs:comment>
    </owl:NamedIndividual>
    


    <!-- http://asi.ice.ucdavis.edu/sustsource/schemas/sustsource.owl#NutritionalStatus -->

    <owl:NamedIndividual rdf:about="&asi;NutritionalStatus">
        <rdf:type rdf:resource="&asi;IntegratedIssue"/>
        <rdf:type rdf:resource="&skos;Concept"/>
        <rdfs:label>Nutritional status</rdfs:label>
        <rdfs:comment>Malnutrition - including under-nutrition, stunting, wasting, or failure to thrive as well as over-consumption; macronutrient sufficiency, micronutrient sufficiency, incidence of nutrition related diseases.</rdfs:comment>
        <skos:related rdf:resource="&asi;Diseases"/>
        <skos:related rdf:resource="&asi;FoodProduction"/>
        <skos:related rdf:resource="&asi;HumanCapital"/>
        <inFramework rdf:resource="&asi;ImpactMitigationFramework"/>
        <skos:related rdf:resource="&asi;Institutions"/>
        <skos:related rdf:resource="&asi;Markets"/>
        <skos:related rdf:resource="&asi;PublicHealth"/>
        <inFramework rdf:resource="&asi;VulnerabilityResilienceFramework"/>
    </owl:NamedIndividual>
    


    <!-- http://asi.ice.ucdavis.edu/sustsource/schemas/sustsource.owl#OceansAndCoasts -->

    <owl:NamedIndividual rdf:about="&asi;OceansAndCoasts">
        <rdf:type rdf:resource="&asi;IntegratedIssue"/>
        <rdf:type rdf:resource="&skos;Concept"/>
        <rdfs:label>Oceans &amp; coasts</rdfs:label>
        <rdfs:comment>Water quality in oceans and coastal areas, ecosystem health of harbors, bays, and estuaries; human populations living in coastal areas, risk of coastal areas to sea level rise due to climate change.</rdfs:comment>
        <skos:related rdf:resource="&asi;AirAndClimate"/>
        <skos:related rdf:resource="&asi;CommonPoolResources"/>
        <skos:related rdf:resource="&asi;EcosystemServices"/>
        <skos:related rdf:resource="&asi;GeographicalDistribution"/>
        <skos:related rdf:resource="&asi;LandAndSoil"/>
        <skos:related rdf:resource="&asi;NaturalCapital"/>
        <skos:related rdf:resource="&asi;ProtectedAreas"/>
    </owl:NamedIndividual>
    


    <!-- http://asi.ice.ucdavis.edu/sustsource/schemas/sustsource.owl#Participation -->

    <owl:NamedIndividual rdf:about="&asi;Participation">
        <rdf:type rdf:resource="&asi;IntegratedIssue"/>
        <rdf:type rdf:resource="&skos;Concept"/>
        <rdfs:label>Participation</rdfs:label>
        <rdfs:comment>Opportunities for and the extent to which producers participate in organizations and institutions in which they can share resources, knowledge, and negotiate collectively. Can include metrics related to participation in cooperatives, unions, or other civil organizations, as well as metrics related to the inclusion of women or underrepresented minority stakeholders in civil society. </rdfs:comment>
        <skos:related rdf:resource="&asi;Governance"/>
        <inFramework rdf:resource="&asi;ImpactMitigationFramework"/>
        <skos:related rdf:resource="&asi;Income"/>
        <skos:related rdf:resource="&asi;Institutions"/>
        <skos:related rdf:resource="&asi;Labor"/>
        <skos:related rdf:resource="&asi;Markets"/>
        <skos:related rdf:resource="&asi;SocialPoliticalCapital"/>
        <inFramework rdf:resource="&asi;VulnerabilityResilienceFramework"/>
    </owl:NamedIndividual>
    


    <!-- http://asi.ice.ucdavis.edu/sustsource/schemas/sustsource.owl#PhysicalCapital -->

    <owl:NamedIndividual rdf:about="&asi;PhysicalCapital">
        <rdf:type rdf:resource="&asi;PhysicalFinancialCapital"/>
        <rdf:type rdf:resource="&skos;Concept"/>
        <rdfs:label>Physical capital</rdfs:label>
        <rdfs:comment>Basic infrastructure and producer goods. Consists of changes to the physical environment such as affordable transport, secure shelter and buildings, adequate water supply and sanitation, clean, affordable energy and access to information (communications), as well as the tools that people use to function more productively (i.e. equipment).</rdfs:comment>
    </owl:NamedIndividual>
    


    <!-- http://asi.ice.ucdavis.edu/sustsource/schemas/sustsource.owl#PhysicalFinancialCapital -->

    <owl:NamedIndividual rdf:about="&asi;PhysicalFinancialCapital">
        <rdf:type rdf:resource="&skos;Concept"/>
        <rdfs:label>Physical &amp; Financial Capital</rdfs:label>
    </owl:NamedIndividual>
    


    <!-- http://asi.ice.ucdavis.edu/sustsource/schemas/sustsource.owl#PoliticalCapital -->

    <owl:NamedIndividual rdf:about="&asi;PoliticalCapital">
        <rdf:type rdf:resource="&asi;SocialPoliticalCapital"/>
        <rdf:type rdf:resource="&skos;Concept"/>
        <rdfs:label>Political capital</rdfs:label>
        <rdfs:comment>Political resources that are key to obtaining or operationalizing rights over other assets. It includes power relations, citizenship, enfranchisement, and membership in political parties.</rdfs:comment>
    </owl:NamedIndividual>
    


    <!-- http://asi.ice.ucdavis.edu/sustsource/schemas/sustsource.owl#PopulationGrowth -->

    <owl:NamedIndividual rdf:about="&asi;PopulationGrowth">
        <rdf:type rdf:resource="&asi;IntegratedIssue"/>
        <rdf:type rdf:resource="&skos;Concept"/>
        <rdfs:label>Population growth</rdfs:label>
        <rdfs:comment>Growth of population in a given region, local to global. Population growth (which can also be negative) interacts with many of the other issues as a driver or outcome.</rdfs:comment>
        <skos:related rdf:resource="&asi;GeographicalDistribution"/>
        <skos:related rdf:resource="&asi;PopulationStructure"/>
        <skos:related rdf:resource="&asi;SocialPoliticalCapital"/>
        <inFramework rdf:resource="&asi;VulnerabilityResilienceFramework"/>
    </owl:NamedIndividual>
    


    <!-- http://asi.ice.ucdavis.edu/sustsource/schemas/sustsource.owl#PopulationStructure -->

    <owl:NamedIndividual rdf:about="&asi;PopulationStructure">
        <rdf:type rdf:resource="&asi;IntegratedIssue"/>
        <rdf:type rdf:resource="&skos;Concept"/>
        <rdfs:label>Population structure</rdfs:label>
        <rdfs:comment>Composition of the population of a given region in terms of age, experience, gender, education, or other variables.</rdfs:comment>
        <skos:related rdf:resource="&asi;GeographicalDistribution"/>
        <skos:related rdf:resource="&asi;PopulationGrowth"/>
        <skos:related rdf:resource="&asi;SocialPoliticalCapital"/>
        <skos:related rdf:resource="&asi;SocialStructure"/>
        <skos:related rdf:resource="&asi;SocioculturalSystems"/>
        <inFramework rdf:resource="&asi;VulnerabilityResilienceFramework"/>
    </owl:NamedIndividual>
    


    <!-- http://asi.ice.ucdavis.edu/sustsource/schemas/sustsource.owl#Poverty -->

    <owl:NamedIndividual rdf:about="&asi;Poverty">
        <rdf:type rdf:resource="&asi;IntegratedIssue"/>
        <rdf:type rdf:resource="&skos;Concept"/>
        <rdfs:label>Poverty</rdfs:label>
        <rdfs:comment>A multi-dimensional condition or outcome that includes deprivation related to human capabilities including consumption and food security, health, education, rights, voice, security, dignity, self-determination, and decent work.</rdfs:comment>
        <skos:related rdf:resource="&asi;HumanRights"/>
        <inFramework rdf:resource="&asi;ImpactMitigationFramework"/>
        <skos:related rdf:resource="&asi;Income"/>
        <skos:related rdf:resource="&asi;Institutions"/>
        <skos:related rdf:resource="&asi;Participation"/>
        <skos:related rdf:resource="&asi;PropertyRights"/>
        <skos:related rdf:resource="&asi;SocialPoliticalCapital"/>
        <skos:related rdf:resource="&asi;SocialStructure"/>
        <inFramework rdf:resource="&asi;VulnerabilityResilienceFramework"/>
        <skos:related rdf:resource="&asi;WomensParticipation"/>
    </owl:NamedIndividual>
    


    <!-- http://asi.ice.ucdavis.edu/sustsource/schemas/sustsource.owl#Productivity -->

    <owl:NamedIndividual rdf:about="&asi;Productivity">
        <rdf:type rdf:resource="&asi;IntegratedIssue"/>
        <rdf:type rdf:resource="&skos;Concept"/>
        <rdfs:label>Productivity</rdfs:label>
        <rdfs:comment>The connection between inputs – both bio-physical and human – and outcomes in agricultural contexts: the net production of agricultural practices. Themes and connected with this issue include crop yields, net farm income, input prices, and efficiency of labor.</rdfs:comment>
        <skos:related rdf:resource="&asi;Income"/>
        <skos:related rdf:resource="&asi;Inputs"/>
        <skos:related rdf:resource="&asi;Labor"/>
        <skos:related rdf:resource="&asi;LandAndSoil"/>
        <skos:related rdf:resource="&asi;SocialPoliticalCapital"/>
        <skos:related rdf:resource="&asi;Technology"/>
        <inFramework rdf:resource="&asi;VulnerabilityResilienceFramework"/>
    </owl:NamedIndividual>
    


    <!-- http://asi.ice.ucdavis.edu/sustsource/schemas/sustsource.owl#PropertyRights -->

    <owl:NamedIndividual rdf:about="&asi;PropertyRights">
        <rdf:type rdf:resource="&asi;IntegratedIssue"/>
        <rdf:type rdf:resource="&skos;Concept"/>
        <rdfs:label>Property rights</rdfs:label>
        <rdfs:comment>Formal and informal rights, policies, and institutions – and the methods, equity, and transparency of enforcement and redress – that characterizes access to and use of land and other resources.</rdfs:comment>
        <skos:related rdf:resource="&asi;Governance"/>
        <skos:related rdf:resource="&asi;HumanRights"/>
        <inFramework rdf:resource="&asi;ImpactMitigationFramework"/>
        <skos:related rdf:resource="&asi;Institutions"/>
        <skos:related rdf:resource="&asi;LandAndSoil"/>
        <skos:related rdf:resource="&asi;SocialPoliticalCapital"/>
        <inFramework rdf:resource="&asi;VulnerabilityResilienceFramework"/>
    </owl:NamedIndividual>
    


    <!-- http://asi.ice.ucdavis.edu/sustsource/schemas/sustsource.owl#ProtectedAreas -->

    <owl:NamedIndividual rdf:about="&asi;ProtectedAreas">
        <rdf:type rdf:resource="&asi;IntegratedIssue"/>
        <rdf:type rdf:resource="&skos;Concept"/>
        <rdfs:label>Protected areas</rdfs:label>
        <rdfs:comment>Land or resources with special status, subject to regulations that restrict human access or resource use. Themes include measures of proportion of land or marine areas in protected status (per given geography), institutional norms of respect for protected area designation, and enforcement of protected status regulations.</rdfs:comment>
        <skos:related rdf:resource="&asi;Biodiversity"/>
        <skos:related rdf:resource="&asi;Governance"/>
        <skos:related rdf:resource="&asi;Institutions"/>
        <skos:related rdf:resource="&asi;LandAndSoil"/>
        <skos:related rdf:resource="&asi;NaturalCapital"/>
        <skos:related rdf:resource="&asi;OceansAndCoasts"/>
    </owl:NamedIndividual>
    


    <!-- http://asi.ice.ucdavis.edu/sustsource/schemas/sustsource.owl#PublicHealth -->

    <owl:NamedIndividual rdf:about="&asi;PublicHealth">
        <rdf:type rdf:resource="&asi;IntegratedIssue"/>
        <rdf:type rdf:resource="&skos;Concept"/>
        <rdfs:label>Public health</rdfs:label>
        <rdfs:comment>The creation and maintenance of the infrastructure, information, capacity, equipment and supplies, and opportunities for the population of a given region to remain in good general health. Themes within this issue include: sanitation, access to reliable safe drinking water, access to healthcare including preventative services, accurate knowledge about nutrition, and food security.</rdfs:comment>
        <skos:related rdf:resource="&asi;Diseases"/>
        <skos:related rdf:resource="&asi;EducationalResources"/>
        <skos:related rdf:resource="&asi;FoodProduction"/>
        <skos:related rdf:resource="&asi;HumanCapital"/>
        <inFramework rdf:resource="&asi;ImpactMitigationFramework"/>
        <skos:related rdf:resource="&asi;NutritionalStatus"/>
        <skos:related rdf:resource="&asi;ReproductiveHealth"/>
        <skos:related rdf:resource="&asi;SocialPoliticalCapital"/>
        <inFramework rdf:resource="&asi;VulnerabilityResilienceFramework"/>
    </owl:NamedIndividual>
    


    <!-- http://asi.ice.ucdavis.edu/sustsource/schemas/sustsource.owl#ReproductiveHealth -->

    <owl:NamedIndividual rdf:about="&asi;ReproductiveHealth">
        <rdf:type rdf:resource="&asi;IntegratedIssue"/>
        <rdf:type rdf:resource="&skos;Concept"/>
        <rdfs:label>Reproductive health</rdfs:label>
        <rdfs:comment>Access to and decision-making authority over family planning, preand post-natal health care. Understanding of and ability to prevent sexually transmitted diseases.</rdfs:comment>
        <skos:related rdf:resource="&asi;Diseases"/>
        <skos:related rdf:resource="&asi;HumanCapital"/>
        <skos:related rdf:resource="&asi;Mortality"/>
        <skos:related rdf:resource="&asi;PublicHealth"/>
    </owl:NamedIndividual>
    


    <!-- http://asi.ice.ucdavis.edu/sustsource/schemas/sustsource.owl#Safety -->

    <owl:NamedIndividual rdf:about="&asi;Safety">
        <rdf:type rdf:resource="&asi;IntegratedIssue"/>
        <rdf:type rdf:resource="&skos;Concept"/>
        <rdfs:label>Safety</rdfs:label>
        <rdfs:comment>The health and safety regulations that ensure safe conditions for agricultural workers. This issue also covers occurrence or risk of accidents in agricultural production systems, and the governmental or corporate responses to accidents.</rdfs:comment>
        <skos:related rdf:resource="&asi;Disasters"/>
        <skos:related rdf:resource="&asi;HumanCapital"/>
        <skos:related rdf:resource="&asi;HumanRights"/>
        <inFramework rdf:resource="&asi;ImpactMitigationFramework"/>
        <skos:related rdf:resource="&asi;Labor"/>
    </owl:NamedIndividual>
    


    <!-- http://asi.ice.ucdavis.edu/sustsource/schemas/sustsource.owl#SocialCapital -->

    <owl:NamedIndividual rdf:about="&asi;SocialCapital">
        <rdf:type rdf:resource="&asi;SocialPoliticalCapital"/>
        <rdf:type rdf:resource="&skos;Concept"/>
        <rdfs:label>Social capital</rdfs:label>
        <rdfs:comment>Social resources that are developed through: 1) networks that build trust and cooperation, including political and civic institutions; 2) membership in groups with rules, norms, and sanctions; and 3) relationships of trust, reciprocity, and exchange that facilitate co-operation, reduce transaction costs, and may provide informal safety nets.</rdfs:comment>
    </owl:NamedIndividual>
    


    <!-- http://asi.ice.ucdavis.edu/sustsource/schemas/sustsource.owl#SocialPoliticalCapital -->

    <owl:NamedIndividual rdf:about="&asi;SocialPoliticalCapital">
        <rdf:type rdf:resource="&asi;Capital"/>
        <rdf:type rdf:resource="&skos;Concept"/>
        <rdfs:label>Social &amp; Political Capital</rdfs:label>
    </owl:NamedIndividual>
    


    <!-- http://asi.ice.ucdavis.edu/sustsource/schemas/sustsource.owl#SocialStructure -->

    <owl:NamedIndividual rdf:about="&asi;SocialStructure">
        <rdf:type rdf:resource="&asi;IntegratedIssue"/>
        <rdf:type rdf:resource="&skos;Concept"/>
        <rdfs:label>Social structure</rdfs:label>
        <rdfs:comment>Aspects of social organization including distribution of power, leadership, and decision-making authority. Includes households, institutions, norms, rules, laws, and policies about management and control of public funds in a given society. Indicators include those related to corruption among other themes.</rdfs:comment>
        <skos:related rdf:resource="&asi;Governance"/>
        <skos:related rdf:resource="&asi;Institutions"/>
        <skos:related rdf:resource="&asi;Participation"/>
        <skos:related rdf:resource="&asi;SocialPoliticalCapital"/>
        <skos:related rdf:resource="&asi;TradePolicies"/>
        <inFramework rdf:resource="&asi;VulnerabilityResilienceFramework"/>
        <skos:related rdf:resource="&asi;WomensParticipation"/>
    </owl:NamedIndividual>
    


    <!-- http://asi.ice.ucdavis.edu/sustsource/schemas/sustsource.owl#SocioculturalSystems -->

    <owl:NamedIndividual rdf:about="&asi;SocioculturalSystems">
        <rdf:type rdf:resource="&asi;IntegratedIssue"/>
        <rdf:type rdf:resource="&skos;Concept"/>
        <rdfs:label>Sociocultural systems</rdfs:label>
        <rdfs:comment>The social and cultural aspects of a given society that shape material assets; economic, political, and social structures; values and norms; and language. Includes systems of ethics, traditional knowledge in agricultural communities, and cultural traditions.</rdfs:comment>
        <inFramework rdf:resource="&asi;ImpactMitigationFramework"/>
        <skos:related rdf:resource="&asi;Institutions"/>
        <skos:related rdf:resource="&asi;PropertyRights"/>
        <skos:related rdf:resource="&asi;SocialPoliticalCapital"/>
        <skos:related rdf:resource="&asi;SocialStructure"/>
        <inFramework rdf:resource="&asi;VulnerabilityResilienceFramework"/>
        <skos:related rdf:resource="&asi;WomensParticipation"/>
    </owl:NamedIndividual>
    


    <!-- http://asi.ice.ucdavis.edu/sustsource/schemas/sustsource.owl#Technology -->

    <owl:NamedIndividual rdf:about="&asi;Technology">
        <rdf:type rdf:resource="&asi;IntegratedIssue"/>
        <rdf:type rdf:resource="&skos;Concept"/>
        <rdfs:label>Technology</rdfs:label>
        <rdfs:comment>Access to, maintenance of, and innovation in technologies including new seed, plant, or livestock varieties, new production technique innovations, information systems, and other tangible innovations. </rdfs:comment>
        <skos:related rdf:resource="&asi;FoodProduction"/>
        <inFramework rdf:resource="&asi;ImpactMitigationFramework"/>
        <skos:related rdf:resource="&asi;Inputs"/>
        <skos:related rdf:resource="&asi;Productivity"/>
        <skos:related rdf:resource="&asi;SocialPoliticalCapital"/>
        <inFramework rdf:resource="&asi;VulnerabilityResilienceFramework"/>
    </owl:NamedIndividual>
    


    <!-- http://asi.ice.ucdavis.edu/sustsource/schemas/sustsource.owl#TradePolicies -->

    <owl:NamedIndividual rdf:about="&asi;TradePolicies">
        <rdf:type rdf:resource="&asi;IntegratedIssue"/>
        <rdf:type rdf:resource="&skos;Concept"/>
        <rdfs:label>Trade policies</rdfs:label>
        <rdfs:comment>The laws, regulations, policies, and norms - locally, regionally, and especially internationally - that govern the trade of agricultural raw materials, and the inputs needed to produce them. This includes public policy as well as private or cooperative trade policies.</rdfs:comment>
        <skos:related rdf:resource="&asi;Governance"/>
        <skos:related rdf:resource="&asi;Institutions"/>
        <skos:related rdf:resource="&asi;Participation"/>
        <skos:related rdf:resource="&asi;SocialPoliticalCapital"/>
        <skos:related rdf:resource="&asi;SocialStructure"/>
        <inFramework rdf:resource="&asi;VulnerabilityResilienceFramework"/>
    </owl:NamedIndividual>
    


    <!-- http://asi.ice.ucdavis.edu/sustsource/schemas/sustsource.owl#VulnerabilityResilienceFramework -->

    <owl:NamedIndividual rdf:about="&asi;VulnerabilityResilienceFramework">
        <rdf:type rdf:resource="&asi;Framework"/>
        <rdf:type rdf:resource="&skos;Concept"/>
        <rdfs:label>Vulnerability/resilience framework</rdfs:label>
    </owl:NamedIndividual>
    


    <!-- http://asi.ice.ucdavis.edu/sustsource/schemas/sustsource.owl#WastesAndPollution -->

    <owl:NamedIndividual rdf:about="&asi;WastesAndPollution">
        <rdf:type rdf:resource="&asi;IntegratedIssue"/>
        <rdf:type rdf:resource="&skos;Concept"/>
        <rdfs:label>Wastes and pollution</rdfs:label>
        <rdfs:comment>Waste management; domestic, agricultural, and industrial effluents; treatment of hazardous wastes, proportion of waste that is recycled or returned to nutrient cycling, emissions of pollutants especially by farming practices, livestock, or other production practices.</rdfs:comment>
        <skos:related rdf:resource="&asi;AirAndClimate"/>
        <skos:related rdf:resource="&asi;EcosystemServices"/>
        <skos:related rdf:resource="&asi;Energy"/>
        <skos:related rdf:resource="&asi;Governance"/>
        <inFramework rdf:resource="&asi;ImpactMitigationFramework"/>
        <skos:related rdf:resource="&asi;NaturalCapital"/>
        <skos:related rdf:resource="&asi;OceansAndCoasts"/>
        <skos:related rdf:resource="&asi;Productivity"/>
        <skos:related rdf:resource="&asi;PublicHealth"/>
        <inFramework rdf:resource="&asi;VulnerabilityResilienceFramework"/>
        <skos:related rdf:resource="&asi;Water"/>
    </owl:NamedIndividual>
    


    <!-- http://asi.ice.ucdavis.edu/sustsource/schemas/sustsource.owl#Water -->

    <owl:NamedIndividual rdf:about="&asi;Water">
        <rdf:type rdf:resource="&asi;IntegratedIssue"/>
        <rdf:type rdf:resource="&skos;Concept"/>
        <rdfs:label>Water</rdfs:label>
        <rdfs:comment>Access to and availability of appropriate quality water across time and space. Refers broadly to water quantity, water quality, annual renewable freshwater resources per capita, sector, or agro-ecological system. Includes access to drinking, cooking, and cleaning water by individuals, as well as issues of access to and use of water for farming: irrigation, ground water, animal hydration, and in primary processing. Can also include water treatment issues (e.g., desalination) and water at larger geographic scale, e.g. watershed health, riparian ecosystem health.</rdfs:comment>
        <skos:related rdf:resource="&asi;CommonPoolResources"/>
        <skos:related rdf:resource="&asi;Diseases"/>
        <skos:related rdf:resource="&asi;EcosystemServices"/>
        <inFramework rdf:resource="&asi;ImpactMitigationFramework"/>
        <skos:related rdf:resource="&asi;Infrastructure"/>
        <skos:related rdf:resource="&asi;LandAndSoil"/>
        <skos:related rdf:resource="&asi;NaturalCapital"/>
        <skos:related rdf:resource="&asi;Productivity"/>
        <skos:related rdf:resource="&asi;PublicHealth"/>
        <inFramework rdf:resource="&asi;VulnerabilityResilienceFramework"/>
        <skos:related rdf:resource="&asi;WastesAndPollution"/>
    </owl:NamedIndividual>
    


    <!-- http://asi.ice.ucdavis.edu/sustsource/schemas/sustsource.owl#WomenAndWages -->

    <owl:NamedIndividual rdf:about="&asi;WomenAndWages">
        <rdf:type rdf:resource="&asi;IntegratedIssue"/>
        <rdf:type rdf:resource="&skos;Concept"/>
        <rdfs:label>Women &amp; wages</rdfs:label>
        <rdfs:comment>The fair and appropriate compensation of women employees, laborers, and all women working in agricultural production. Includes employment opportunities and business or farm ownership opportunities for women.</rdfs:comment>
        <skos:related rdf:resource="&asi;HumanRights"/>
        <inFramework rdf:resource="&asi;ImpactMitigationFramework"/>
        <skos:related rdf:resource="&asi;Income"/>
        <skos:related rdf:resource="&asi;Labor"/>
        <skos:related rdf:resource="&asi;Poverty"/>
        <skos:related rdf:resource="&asi;PropertyRights"/>
        <skos:related rdf:resource="&asi;SocialPoliticalCapital"/>
        <skos:related rdf:resource="&asi;SocialStructure"/>
    </owl:NamedIndividual>
    


    <!-- http://asi.ice.ucdavis.edu/sustsource/schemas/sustsource.owl#WomensParticipation -->

    <owl:NamedIndividual rdf:about="&asi;WomensParticipation">
        <rdf:type rdf:resource="&asi;IntegratedIssue"/>
        <rdf:type rdf:resource="&skos;Concept"/>
        <rdfs:label>Women&apos;s participation</rdfs:label>
        <rdfs:comment>Women&apos;s engagement and opportunities for engagement in political, cultural, legal, and economic decision making groups. Includes opportunities for farm and business ownership or management. Metrics include the number of women who are part of unions or cooperatives, the number of women business owners, and proportion of women on decision making boards at multiple levels of society.</rdfs:comment>
        <skos:related rdf:resource="&asi;Income"/>
        <skos:related rdf:resource="&asi;Institutions"/>
        <skos:related rdf:resource="&asi;PropertyRights"/>
        <skos:related rdf:resource="&asi;SocialPoliticalCapital"/>
        <skos:related rdf:resource="&asi;SocialStructure"/>
        <skos:related rdf:resource="&asi;SocioculturalSystems"/>
        <skos:related rdf:resource="&asi;WomenAndWages"/>
    </owl:NamedIndividual>
</rdf:RDF>



<!-- Generated by the OWL API (version 3.3.1957) http://owlapi.sourceforge.net -->

